Notations, correction typing rule while, stdpp

theories/main.v
@@ -1,26 +1,26 @@
-
 Require Import String.
 From Coq Require Import Streams.
 From Coq Require Import Lists.List.
+From stdpp Require Import gmap.
+(* Import ListNotations. *)
 Open Scope string_scope.
 Require Import ssreflect.
+From fspini Require Import map_simpl.
 
 
 Inductive op :=
 | Add | Sub | Mul | Eq | Neq | Leq | Lt | Geq | Gt.
 
-Definition var := string.
-Definition value := nat.
+Notation var := string.
+Notation value := nat.
 
 Inductive expr :=
 | ELit : value -> expr
 | EVar : var -> expr
 | EOp : expr -> op -> expr -> expr.
 
-
 Inductive channel :=
   Public | Secret.
-
 
 Inductive command :=
 | CSkip : command
@@ -32,41 +32,52 @@ Inductive command :=
 | COutput : channel -> expr -> command
 .
 
+Coercion ELit: value >-> expr.
+Coercion EVar: var >-> expr.
+
+Notation "'SKIP'" := CSkip.
+Notation "x '::=' e" :=(CAssign x e) (at level 60).
+Notation "c1 ;;; c2" :=
+  (CSeq c1 c2) (at level 80, right associativity).
+Notation "'WHILE' b 'DO' c 'END'" :=
+  (CWhile b c) (at level 80, right associativity).
+Notation "'IFB' c1 'THEN' c2 'ELSE' c3 'FI'" :=
+  (CIfThenElse c1 c2 c3) (at level 80, right associativity).
+Notation "'INPUT' x '@' c" := (CInput c x) (at level 60).
+Notation "'OUTPUT' e '@' c" := (COutput c e) (at level 60).
 
 (* This type will be used for both memories and contexts *)
-Inductive varmap (A : Type) :=
-| Empty : varmap A
-| Cons : var -> A -> varmap A -> varmap A
-.
+(* Inductive varmap (A : Type) := *)
+(* | Empty : varmap A *)
+(* | Cons : var -> A -> varmap A -> varmap A *)
+(* . *)
 
+(* Fixpoint find_var {A} x (m : varmap A) := *)
+(*   match m with *)
+(*   | Empty _ => None *)
+(*   | Cons _ y v m => if String.eqb y x then Some v else find_var x m *)
+(*   end. *)
 
+(* Fixpoint find_and_remove {A} x (m : varmap A) := *)
+(*   match m with *)
+(*   | Empty _ => None *)
+(*   | Cons _ y v m => if String.eqb y x then Some (v, m) else *)
+(*                      match find_and_remove x m with *)
+(*                      | None => None *)
+(*                      | Some (vx, m) => Some (vx, Cons _ y v m) *)
+(*                      end *)
+(*   end. *)
 
-Fixpoint find_var {A} x (m : varmap A) :=
-  match m with
-  | Empty _ => None
-  | Cons _ y v m => if String.eqb y x then Some v else find_var x m
-  end.
+(* Fixpoint set_var {A} x (v : A) m := *)
+(*   match m with *)
+(*   | Empty _ => Cons _ x v m *)
+(*   | Cons _ y vy m => if String.eqb y x then Cons _ x v m else Cons _ y vy (set_var x v m) *)
+(*   end. *)
 
-Fixpoint find_and_remove {A} x (m : varmap A) :=
-  match m with
-  | Empty _ => None
-  | Cons _ y v m => if String.eqb y x then Some (v, m) else
-                     match find_and_remove x m with
-                     | None => None
-                     | Some (vx, m) => Some (vx, Cons _ y v m)
-                     end
-  end.
+(* Notation "'[' x ':=' v ']' m" := (Cons _ x v m) (at level 40). *)
+(* Notation "'∅'" := (Empty _) (at level 40). *)
 
-Fixpoint set_var {A} x (v : A) m :=
-  match m with
-  | Empty _ => Cons _ x v m
-  | Cons _ y vy m => if String.eqb y x then Cons _ x v m else Cons _ y vy (set_var x v m)
-  end.
-
-
-
-Definition memory := varmap value.
-
+Definition memory := gmap var value.
 
 Fixpoint apply_op (l : value) op r : value :=
   match op with
@@ -82,101 +93,116 @@ Fixpoint apply_op (l : value) op r : value :=
   end .
 
 
-
 Inductive eval_expr : expr -> memory -> value -> Prop :=
 | Lit : forall n m, eval_expr (ELit n) m n
-| Var : forall x m v, find_var x m = Some v -> eval_expr (EVar x) m v
+| Var : forall x m v, m !! x = Some v -> eval_expr (EVar x) m v
 | Op : forall e1 op e2 v1 v2 m, eval_expr e1 m v1 -> eval_expr e2 m v2 ->
                            eval_expr (EOp e1 op e2) m (apply_op v1 op v2)
 .
+
+Notation "e ';' m '⇓' v" := (eval_expr e m v) (at level 20).
+Notation "x :::: c" := (Streams.Cons x c) (at level 20).
 
 Inductive event :=
 | EvInput : channel -> value -> event
 | EvOutput : channel -> value -> event.
 Definition trace := list event.
 (* In the state, Some c represents a command, and None represents a Skip *)
-Definition state : Type := (Stream value) * (Stream value) * (option command) * memory * trace.
+Definition state : Type := (Stream value) * (Stream value) * memory * trace.
+Inductive config := Config (c : option command) ( st : state).
+Notation "'⟪' c ',' st '⟫'" := (Config c st) (at level 10, c at level 20, st at level 20).
 
+Reserved Notation "cfg '--->' cfg'" (at level 40).
+Inductive exec_command : config -> config -> Prop :=
+| Skip : forall st,
+  ⟪ Some SKIP , st ⟫ ---> ⟪ None , st ⟫
 
-Inductive exec_command : state -> state -> Prop :=
-| Skip : forall S P m t,
-    exec_command (S, P, Some CSkip, m, t) (S, P, None, m, t)
 | Assign : forall S P x e v m t,
-    eval_expr e m v ->
-    exec_command (S, P, Some (CAssign x e), m, t) (S, P, None, set_var x v m, t)
-| Seq1 : forall S P c1 c2 m t S' P' c1' m' t',
-    exec_command (S, P, Some c1, m, t) (S', P', Some c1', m', t') ->
-    exec_command (S, P, Some (CSeq c1 c2), m, t) (S', P', Some (CSeq c1' c2), m', t')
-| Seq2 : forall S P c1 c2 m t S' P' m' t',
-    exec_command (S, P, Some c1, m, t) (S', P', None, m', t') ->
-    exec_command (S, P, Some (CSeq c1 c2), m, t) (S', P', Some c2, m', t')
-| If : forall S P e (c1 : command) c2 m t v (c: command),
-    eval_expr e m v ->
-    c = (if Nat.eqb v 0 then c2 else c1) ->
-    exec_command (S, P, Some (CIfThenElse e c1 c2), m, t) (S, P, Some c, m, t)
-| While : forall S P e c m t,
-    exec_command (S, P, Some (CWhile e c), m, t)
-      (S, P, Some (CIfThenElse e (CSeq c (CWhile e c)) CSkip), m, t)
+  e ; m ⇓ v ->
+  ⟪ Some (x ::= e), (S, P, m, t) ⟫ ---> ⟪ None , (S, P, <[ x := v ]> m, t) ⟫
+
+| Seq1 : forall st c1 c2 st' c1',
+  ⟪ Some c1 , st ⟫ ---> ⟪ Some c1' , st' ⟫ ->
+  ⟪ Some (c1 ;;; c2) , st ⟫ ---> ⟪ Some (c1' ;;; c2) , st' ⟫
+
+| Seq2 : forall st c1 c2 st',
+  ⟪ Some c1 , st ⟫ ---> ⟪ None , st' ⟫ ->
+  ⟪ Some (c1 ;;; c2) , st ⟫ ---> ⟪ Some c2 , st' ⟫
+
+| If : forall S P e (c1 c2 : command) m t v (c: command),
+  e ; m ⇓ v ->
+  c = (if Nat.eqb v 0 then c2 else c1) ->
+  ⟪ Some (IFB e THEN c1 ELSE c2 FI), (S, P, m, t) ⟫ ---> ⟪ Some c, (S, P, m, t) ⟫
+
+| While : forall st c e,
+  ⟪ Some (WHILE e DO c END) , st ⟫ --->
+  ⟪ Some (IFB e THEN (c ;;; WHILE e DO c END) ELSE SKIP FI) , st ⟫
+
 | InputPublic : forall S v P x m t,
-    exec_command (S, Streams.Cons v P, Some (CInput Public x), m, t)
-      (S, P, None, set_var x v m, EvInput Public v :: t)
+  ⟪ Some (INPUT x @Public) , (S, v::::P, m, t) ⟫ --->
+  ⟪ None , (S, P, <[ x := v ]> m, EvInput Public v :: t) ⟫
+
 | InputSecret : forall v S P x m t,
-    exec_command (Streams.Cons v S, P, Some (CInput Secret x), m, t)
-      (S, P, None, set_var x v m, EvInput Secret v :: t)
+  ⟪ Some (INPUT x @Secret) , (v::::S, P, m, t) ⟫ --->
+  ⟪ None , (S, P, <[ x := v ]> m, EvInput Secret v :: t) ⟫
+
 | Output : forall S P ch e m t v,
-    eval_expr e m v ->
-    exec_command (S, P, Some (COutput ch e), m, t) (S, P, None, m, EvOutput ch v :: t)
-.
+  e ; m ⇓ v ->
+  ⟪ Some (OUTPUT e @ch) , (S, P, m, t) ⟫ --->
+  ⟪ None , (S, P, m, EvOutput ch v :: t) ⟫
+where "cfg '--->' cfg'" := (exec_command cfg cfg').
 
 
 (* reflexive and transitive closure of the execution relation: *)
-Inductive exec_trans : state -> state -> Prop :=
-| exec_empty : forall s, exec_trans s s
-| exec_step : forall s1 s2 s3, exec_command s1 s2 -> exec_trans s2 s3 -> exec_trans s1 s3
-.
+Definition exec_trans : config -> config -> Prop := rtc exec_command.
+Notation "cfg '--->*' cfg'" := (exec_trans cfg cfg') (at level 40).
+(* | exec_empty : forall s, exec_trans s s *)
+(* | exec_step : forall s1 s2 s3, exec_command s1 s2 -> exec_trans s2 s3 -> exec_trans s1 s3 *)
+(* . *)
 
 (* Initial memory *)
-Definition minit := Empty value.
+Definition minit : memory := gmap_empty.
 
-Fixpoint public_projection (t: trace) :=
+Fixpoint public_projection (t: trace) : trace :=
   match t with
-  | nil => nil
-  | EvInput Public v :: q => EvInput Public v :: public_projection q
-  | EvOutput Public v ::q => EvOutput Public v :: public_projection q
-  | _ :: q => public_projection q
+  | [] => []
+  | (EvInput Public v) :: q => (EvInput Public v :: public_projection q)
+  | (EvOutput Public v) :: q => (EvOutput Public v :: public_projection q)
+  | _ :: q => (public_projection q)
   end.
 
 
 (* knowledge P c d S means that S is in the Set K(P,c,d) *)
 Inductive knowledge: (Stream value) -> command -> trace -> (Stream value) -> Prop :=
 | Know : forall P c d S,
-    (exists S' P' c' m' t', exec_trans (S, P, Some c, minit, nil) (S', P', c', m', t') /\
-                         public_projection t' = d) ->
-    knowledge P c d S
+    (exists S' P' c' m' t',
+        ⟪ Some c, (S, P, minit, nil) ⟫ --->* ⟪ c' ,  (S', P', m', t') ⟫
+        /\ public_projection t' = d)
+    -> knowledge P c d S
 .
-
 
 Definition PSNI c :=
   forall P a d t,
-    (exists S S' P' c' m', exec_trans (S, P, Some c, minit, nil) (S', P', c', m', t) /\
-                        public_projection t = a :: d) ->
+    (exists S S' P' c' m',
+        ⟪ Some c, (S, P, minit, nil) ⟫ --->* ⟪ c' ,  (S', P', m', t) ⟫
+        /\ public_projection t = a :: d) ->
     (* Set equality is described with an iff *)
     (forall S, knowledge P c (a :: d) S <-> knowledge P c d S).
-
 
 (* progress_knowledge P c d S means that S is in the Set K->(P,c,d) *)
 Inductive progress_knowledge: (Stream value) -> command -> trace -> (Stream value) -> Prop :=
 | PKnow : forall P c d S,
-    (exists S' P' c' m' t' a, exec_trans (S, P, Some c, minit, nil) (S', P', c', m', t') /\
-                           public_projection t' = a :: d) ->
+    (exists S' P' c' m' t' a,
+        ⟪ Some c, (S, P, minit, nil) ⟫ --->* ⟪ c' ,  (S', P', m', t') ⟫
+        /\ public_projection t' = a :: d) ->
     progress_knowledge P c d S
 .
 
-
 Definition PINI c :=
   forall P a d t,
-    (exists S S' P' c' m', exec_trans (S, P, Some c, minit, nil) (S', P', c', m', t) /\
-                        public_projection t = a :: d) ->
+    (exists S S' P' c' m',
+        ⟪ Some c, (S, P, minit, nil) ⟫ --->* ⟪ c' ,  (S', P', m', t) ⟫
+        /\ public_projection t = a :: d) ->
     (* Set equality is described with an iff *)
     (forall S, knowledge P c (a :: d) S <-> progress_knowledge P c d S).
 
@@ -196,42 +222,63 @@ Definition flows l1 l2 :=
   | _, _ => True
   end.
 
-Definition context := varmap confidentiality.
-Definition gamma0 := Empty confidentiality.
+#[export] Instance sqsubseteq_confidentiality : SqSubsetEq confidentiality.
+Proof. exact flows. Defined.
+
+#[export] Instance join_confidentiality : Join confidentiality.
+Proof. exact join. Defined.
+
+(* Notation "l1 '⊔' l2" := (join l1 l2) (at level 40). *)
+(* Notation "l1 '⊑' l2" := (flows l1 l2) (at level 40). *)
+
+Definition context := gmap var confidentiality.
+Definition gamma0 : context := gmap_empty.
 
 (* A memory and a context have the same support if the same variables are defined in them *)
 Definition same_support (m : memory) (gamma : context) : Prop :=
-  forall x, match find_var x m, find_var x gamma with
+  forall x, match m !! x, gamma !! x with
        | Some _, Some _ | None, None => True
        | _, _ => False
        end.
 
 
-
 (* Joining two contexts, to be used after an If-statement *)
-Fixpoint join_context (gamma1 gamma2 : context) : context :=
-  match gamma1 with
-  | Empty _ => gamma2
-  | Cons _ x v gamma1 =>
-      match find_and_remove x gamma2 with
-      | Some (v', gamma2) => Cons _ x (join v v') (join_context gamma1 gamma2)
-      | None => Cons _ x v (join_context gamma1 gamma2)
-      end
-  end.
+(* Fixpoint join_context (gamma1 gamma2 : context) : context := *)
+(*   match gamma1 with *)
+(*   | Empty _ => gamma2 *)
+(*   | Cons _ x v gamma1 => *)
+(*       match find_and_remove x gamma2 with *)
+(*       | Some (v', gamma2) => Cons _ x (join v v') (join_context gamma1 gamma2) *)
+(*       | None => Cons _ x v (join_context gamma1 gamma2) *)
+(*       end *)
+(*   end. *)
+
+Definition join_context (gamma1 gamma2 : context) : context :=
+  gmap_merge _ _ _
+    (fun opt1 opt2 =>
+       match opt1, opt2 with
+       | Some l1, Some l2 => Some (l1 ⊔ l2)
+       | None, _ => opt2
+       | _, None => opt1
+       end
+    )
+    gamma1 gamma2.
+Notation "g1 '⊔g' g2" := (join_context g1 g2) (at level 40).
+
+Reserved Notation "'{{' Γ '⊢' e ':' ℓ '}}'" (at level 10, Γ at level 50, e at level 99).
 
 Inductive typecheck_expr : context -> expr -> confidentiality -> Prop :=
-| TLit : forall gamma n,
-    typecheck_expr gamma (ELit n) LPublic
-| TVar : forall l gamma x,
-    find_var x gamma = Some l ->
-    typecheck_expr gamma (EVar x) l
-| TOp : forall l1 l2 gamma e1 op e2 l,
-    typecheck_expr gamma e1 l1 ->
-    typecheck_expr gamma e2 l2 ->
-    l = join l1 l2 ->
-    typecheck_expr gamma (EOp e1 op e2) l
+| TLit : forall Γ n, {{ Γ ⊢ (ELit n) : LPublic }}
+| TVar : forall l Γ x,
+     Γ !! x = Some l ->
+    {{ Γ ⊢ (EVar x) : l }}
+| TOp : forall l1 l2 Γ e1 op e2 l,
+    {{ Γ ⊢ e1 : l1 }} ->
+    {{ Γ ⊢ e2 : l2 }} ->
+    l = (l1 ⊔ l2) ->
+    {{ Γ ⊢ (EOp e1 op e2) : l }}
+where "{{ Γ '⊢' e ':' ℓ }}" := (typecheck_expr Γ e ℓ)
 .
-
 
 Definition confidentiality_of_channel ch :=
   match ch with
@@ -239,48 +286,66 @@ Definition confidentiality_of_channel ch :=
   | Public => LPublic
   end.
 
+Reserved Notation "-{ Γ ',' pc '⊢' e '~>' Γ2 }-"
+  (at level 10, Γ at level 55, Γ2 at level 50, pc at level 35, e at level 99).
 Inductive typecheck : context -> confidentiality -> command -> context -> Prop :=
-| TSkip : forall gamma pc,
-    typecheck gamma pc CSkip gamma
-| TAssign : forall le gamma pc x e gamma',
-    typecheck_expr gamma e le ->
-    gamma' = set_var x (join le pc) gamma ->
-    typecheck gamma pc (CAssign x e) gamma'
-| TSeq : forall gamma1 gamma2 gamma3 pc c1 c2,
-    typecheck gamma1 pc c1 gamma2 ->
-    typecheck gamma2 pc c2 gamma3 ->
-    typecheck gamma1 pc (CSeq c1 c2) gamma3
-| TIf : forall l gamma gamma1 gamma2 gamma' pc e c1 c2,
-    typecheck_expr gamma e l ->
-    typecheck gamma (join pc l) c1 gamma1 ->
-    typecheck gamma (join pc l) c2 gamma2 ->
-    gamma' = join_context gamma1 gamma2 ->
-    typecheck gamma pc (CIfThenElse e c1 c2) gamma'
-| TWhile : forall l gamma pc e c gamma',
-    typecheck_expr gamma e l ->
-    typecheck gamma (join pc l) c gamma' ->
-    typecheck gamma pc (CWhile e c) gamma'
-| TInput : forall gamma pc x ch gamma',
-    flows pc (confidentiality_of_channel ch) ->
-    gamma' = set_var x (join (confidentiality_of_channel ch) pc) gamma ->
-    typecheck gamma pc (CInput ch x) gamma'
-| TOutput : forall le gamma pc e ch,
-    typecheck_expr gamma e le ->
-    flows (join pc le) (confidentiality_of_channel ch) ->
-    typecheck gamma pc (COutput ch e) gamma
+| TSkip : forall Γ pc,
+  -{ Γ, pc ⊢ CSkip ~> Γ }-
+
+| TAssign : forall le Γ pc x e Γ',
+  {{ Γ ⊢ e : le }} ->
+  Γ' = <[ x := (le ⊔ pc) ]> Γ ->
+  -{ Γ, pc ⊢ (CAssign x e) ~> Γ' }-
+
+| TSeq : forall (Γ1 Γ2 Γ3 : context) pc c1 c2,
+  -{ Γ1, pc ⊢ c1 ~> Γ2 }- ->
+  -{ Γ2, pc ⊢ c2 ~> Γ3 }- ->
+  -{ Γ1, pc ⊢ (CSeq c1 c2) ~> Γ3 }-
+
+| TIf : forall l Γ Γ1 Γ2 Γ' pc e c1 c2,
+  {{ Γ ⊢ e : l }} ->
+  -{ Γ, pc ⊔ l ⊢ c1 ~> Γ1 }- ->
+  -{ Γ, pc ⊔ l ⊢ c2 ~> Γ2 }- ->
+  Γ' = (Γ1 ⊔g Γ2) ->
+  -{ Γ, pc ⊢ (CIfThenElse e c1 c2) ~> Γ' }-
+
+(* Does not change the environment *)
+| TWhile1 : forall l Γ pc e c,
+  {{ Γ ⊢ e : l }} ->
+  -{ Γ, pc ⊔ l ⊢ c ~> Γ }- ->
+  -{ Γ, pc ⊢ (CWhile e c) ~> Γ }-
+
+(* Does change the environment *)
+| TWhile2 : forall l Γ pc e c Γ' Γ'',
+  {{ Γ ⊢ e : l }} ->
+  -{ Γ, pc ⊔ l ⊢ c ~> Γ'' }- ->
+  -{ Γ'', pc ⊢ (CWhile e c) ~> Γ' }- ->
+  -{ Γ, pc ⊢ (CWhile e c) ~> Γ' }-
+
+| TInput : forall Γ pc x ch Γ',
+  (pc ⊑ confidentiality_of_channel ch) ->
+  Γ' = <[ x := ((confidentiality_of_channel ch) ⊔ pc) ]> Γ ->
+  -{ Γ, pc ⊢ (CInput ch x) ~> Γ' }-
+
+| TOutput : forall le Γ pc e ch,
+  {{ Γ ⊢ e : le }} ->
+  ((pc ⊔ le) ⊑ confidentiality_of_channel ch) ->
+  -{ Γ, pc ⊢ (COutput ch e) ~> Γ }-
+where "-{ Γ ',' pc '⊢' e '~>' Γ2 }-" := (typecheck Γ pc e Γ2)
 .
 
 
-
+(** Examples *)
+Definition example_typecheck example := exists gamma, -{ ∅ , LPublic ⊢ example ~> gamma}-.
 (* /* Program 1 -- should be well-typed as it satisfies PINI (and PSNI) */ *)
 (* input(secret, x) *)
 (* x = 0 *)
 (* output(public, x) *)
 Definition example1 :=
-  CSeq (CInput Secret "x")
-       (CSeq (CAssign "x" (ELit 0)) (COutput Public (EVar "x"))).
+ (INPUT "x" @Secret) ;;;
+   ("x" ::= 0) ;;;
+   (OUTPUT "x" @Public).
 
-Definition example_typecheck example := exists gamma, typecheck (Empty _) LPublic example gamma.
 Lemma example1_typecheck : example_typecheck example1.
 Proof.
   eexists.
@@ -291,7 +356,7 @@ Qed.
 (* input(secret, x) *)
 (* output(public, x) *)
 Definition example2 :=
-  CSeq (CInput Secret "x") (COutput Public (EVar "x")).
+  (INPUT "x" @Secret) ;;; (OUTPUT "x" @Public).
 Lemma example2_not_typecheck : not (example_typecheck example2).
 Proof.
   intro.
@@ -315,19 +380,11 @@ Qed.
 (* output(public, y) *)
 
 Definition example3 :=
-  CSeq
-    (CInput Secret "x")
-    (CSeq
-       (CAssign "y" (ELit 0))
-       (CSeq
-       (CIfThenElse
-          (EVar "x")
-          (CAssign "y" (ELit 1))
-          (CSkip)
-       )
-       (COutput Public (EVar "y"))
-       )
-    ).
+  INPUT "x" @Secret ;;;
+  "y" ::= 0 ;;;
+  IFB "x" THEN "y" ::= 1 ELSE SKIP FI ;;;
+  OUTPUT "y" @Public.
+
 Lemma example3_not_typecheck : not (example_typecheck example3).
 Proof.
   intro.
@@ -363,27 +420,15 @@ Qed.
 (* y = 0 *)
 (* output(public, y) *)
 Definition example4 :=
-  CSeq
-    (CInput Secret "x")
-    (CSeq
-       (CIfThenElse
-          (EVar "x")
-          (CAssign "y" (ELit 1))
-          (CSkip)
-       )
-       (CSeq
-          (COutput Secret (EVar "y"))
-          (CSeq
-             (CAssign "y" (ELit 0))
-             (COutput Public (EVar "y"))
-          )
-       )
-    ).
+  INPUT "x" @Secret ;;;
+  IFB "x" THEN "y" ::= 1 ELSE SKIP FI ;;;
+  OUTPUT "y" @Secret ;;;
+  "y" ::= 0 ;;;
+  OUTPUT "y" @Public.
 Lemma example4_typecheck : example_typecheck example4.
 Proof.
   repeat econstructor.
 Qed.
-
 
 (* /* Program 5 -- should be well-typed as it satisfies PINI */ *)
 (* input(secret, x) *)
@@ -392,21 +437,27 @@ Qed.
 (*    input(secret, y) *)
 (* output(public, 0) *)
 Definition example5 :=
-  CSeq
-    (CInput Secret "x")
-    (CSeq
-       (CWhile
-          (EVar "x")
-          (CSeq
-             (CAssign "x" (EOp (EVar "x") Sub (ELit 1)))
-             (CInput Secret "y")
-          )
-       )
-       (COutput Public (ELit 0))
-    ).
+  INPUT "x" @Secret ;;;
+  ( WHILE "x"
+      DO
+      "x" ::= (EOp "x" Sub 1);;;
+      INPUT "y" @Secret
+      END
+  ) ;;;
+  OUTPUT 0 @Public.
+
 Lemma example5_typecheck : example_typecheck example5.
 Proof.
-  repeat econstructor.
+  econstructor.
+  econstructor.
+  econstructor.
+  econstructor.
+  eauto.
+  econstructor.
+  eapply TWhile2.
+  all : (repeat econstructor).
+  cbn.
+  by repeat (symmetry; map_simpl).
 Qed.
 
 (* /* Program 6 -- must be ill-typed as it violates PINI */ *)
@@ -416,18 +467,14 @@ Qed.
 (* input(secret, y) *)
 (* output(public, x) *)
 Definition example6 :=
-  CSeq
-    (CInput Secret "x")
-    (CSeq
-       (CWhile
-          (EVar "x")
-          (CSeq
-             (CAssign "x" (EOp (EVar "x") Sub (ELit 1)))
-             (CInput Secret "y")
-          )
-       )
-       (COutput Public (EVar "x"))
-    ).
+    INPUT "x" @Secret ;;;
+    ( WHILE "x"
+        DO
+        "x" ::= (EOp "x" Sub 1);;;
+        INPUT "y" @Secret
+        END
+    ) ;;;
+    OUTPUT "x" @Public.
 Lemma example6_typecheck : not (example_typecheck example6).
 Proof.
   intro.
@@ -438,89 +485,224 @@ Proof.
   inversion H6;subst; clear H6.
 
   inversion H4;subst; clear H4.
-  inversion H9;subst; clear H9.
-  inversion H4;subst; clear H4.
-  inversion H7;subst; clear H7.
-  inversion H10;subst; clear H10.
-  inversion H5;subst; clear H5.
-  inversion H6;subst; clear H6.
-  inversion H4;subst; clear H4.
-  inversion H11;subst; clear H11.
-  cbn in *. inversion H3; inversion H5 ; subst.
-  cbn in H2; inversion H2; subst.
-  by cbn in H8.
-Qed.
+  - inversion H9;subst; clear H9.
+    inversion H4;subst; clear H4.
+    inversion H7;subst; clear H7.
+    inversion H10;subst; clear H10.
+    inversion H5;subst; clear H5.
+    inversion H6;subst; clear H6.
+    inversion H4;subst; clear H4.
+    inversion H11;subst; clear H11.
+    cbn in *. inversion H3; inversion H5 ; subst.
+    cbn in H2; inversion H2; subst.
+    by cbn in H8.
+  - admit.
+Admitted.
 
 (* /* Program 7 -- must be well-typed  */ *)
 (* input(secret, x) *)
 (* input(public, x) *)
 (* output(public, x) *)
 Definition example7 :=
-  (CSeq
-     (CInput Secret "x")
-     (CSeq
-        (CInput Public "x")
-        (COutput Public (EVar "x"))
-     )
-  ).
+  INPUT "x" @Secret ;;;
+  INPUT "x" @Public ;;;
+  OUTPUT "x" @Public
+  .
 Lemma example7_typecheck : example_typecheck example7.
 Proof.
   repeat econstructor.
 Qed.
 
 
+(* /* Program 8 -- must be ill-typed  */ *)
+(* input(public, x); *)
+(* while x: *)
+(*   output(public, x); *)
+(*   input(secret, x) *)
 
+Definition example8 :=
+  INPUT "x" @Public ;;;
+  ( WHILE "x"
+      DO
+      OUTPUT "x" @Public;;;
+      INPUT "x" @Secret
+      END
+  ).
+Lemma example8_typecheck : not (example_typecheck example8).
+Proof.
+Admitted.
 
+(* Inductive pevent : Type := *)
+(* | EmptyEvent *)
+(* | AssignEvent (x : var) (v : value) *)
+(* | InputEvent (v : value) *)
+(* | OutputEvent (v : value) *)
+(* . *)
 
+(* Inductive event_step : state -> context -> confidentiality -> pevent -> state -> context -> confidentiality -> Prop:= *)
+(* | PSkip : forall S P m t gamma pc, *)
+(*   exec_command (S, P, Some CSkip, m, t) (S, P, None, m, t) -> *)
+(*   event_step (S, P, Some CSkip, m, t) gamma pc EmptyEvent (S, P, None, m, t) gamma pc *)
 
+(* | PAssignPublic : forall S P x e v m t gamma pc gamma' l, *)
+(*   exec_command (S, P, Some (CAssign x e), m, t) (S, P, None, set_var x v m, t) -> *)
+(*   eval_expr e m v -> *)
+(*   find_var x gamma = Some l -> (* We REQUIRE that x has the right label *) *)
+(*   gamma' = set_var x (l ⊔ pc) gamma -> *)
+(*   event_step (S, P, Some (CAssign x e), m, t) gamma pc *)
+(*     (AssignEvent x v) (S, P, None, set_var x v m, t) gamma' pc *)
 
+(* (* TODO When doing the sequence, the level of the pc never change... *)
+(*    Only when we enter enter in a block, but seq stays at the same level *) *)
+(* | PSeq1 : forall S P c1 c2 m t S' P' c1' m' t' ev gamma pc gamma', *)
+(*   exec_command (S, P, Some (CSeq c1 c2), m, t) (S', P', Some (CSeq c1' c2), m', t') -> *)
+(*   event_step *)
+(*     (S, P, Some c1, m, t) gamma pc *)
+(*     ev *)
+(*     (S', P', Some c1', m', t') gamma' pc -> *)
+(*   event_step *)
+(*     (S, P, Some (CSeq c1 c2), m, t) gamma pc *)
+(*     ev *)
+(*     (S', P', Some (CSeq c1' c2), m', t') *)
+(*     gamma' pc *)
 
+(* | PSeq2 : forall S P c1 c2 m t S' P' m' t' ev gamma gamma' pc, *)
+(*   exec_command (S, P, Some (CSeq c1 c2), m, t) (S', P', Some c2, m', t') -> *)
+(*   event_step (S, P, Some c1, m, t) gamma pc ev (S', P', None, m', t') gamma' pc -> *)
+(*   event_step (S, P, Some (CSeq c1 c2), m, t) gamma pc ev (S', P', Some c2, m', t') gamma' pc *)
 
+(* | PIf : forall S P e (c1 : command) c2 m t v (c: command) l gamma pc, *)
+(*   exec_command *)
+(*     (S, P, Some (CIfThenElse e c1 c2), m, t) *)
+(*     (S, P, Some c, m, t) -> *)
+(*   eval_expr e m v -> *)
+(*   typecheck_expr gamma e l -> *)
+(*   c = (if Nat.eqb v 0 then c2 else c1) -> *)
+(*   event_step *)
+(*     (S, P, Some (CIfThenElse e c1 c2), m, t) gamma pc *)
+(*     EmptyEvent *)
+(*     (S, P, Some c, m, t) gamma (pc ⊔ l) *)
 
+(* | PWhile : forall S P e c m t, *)
+(*   exec_command *)
+(*     (S, P, Some (CWhile e c), m, t) *)
+(*     (S, P, Some (CIfThenElse e (CSeq c (CWhile e c)) CSkip), m, t) -> *)
+(*   event_step *)
+(*     (S, P, Some (CWhile e c), m, t) *)
+(*     EmptyEvent *)
+(*     (S, P, Some (CIfThenElse e (CSeq c (CWhile e c)) CSkip), m, t) *)
 
+(* | PInputPublic : forall S v P x m t, *)
+(*   exec_command *)
+(*     (S, Streams.Cons v P, Some (CInput Public x), m, t) *)
+(*     (S, P, None, set_var x v m, EvInput Public v :: t) -> *)
+(*   event_step *)
+(*     (S, Streams.Cons v P, Some (CInput Public x), m, t) *)
+(*     (InputEvent v) *)
+(*     (S, P, None, set_var x v m, EvInput Public v :: t) *)
+
+(* | PInputSecret : forall v S P x m t, *)
+(*   exec_command *)
+(*     (Streams.Cons v S, P, Some (CInput Secret x), m, t) *)
+(*     (S, P, None, set_var x v m, EvInput Secret v :: t) -> *)
+(*   event_step *)
+(*     (Streams.Cons v S, P, Some (CInput Secret x), m, t) *)
+(*     EmptyEvent *)
+(*     (S, P, None, set_var x v m, EvInput Secret v :: t) *)
+
+(* | POutputPublic : forall S P e m t v, *)
+(*   exec_command (S, P, Some (COutput Public e), m, t) (S, P, None, m, EvOutput Public v :: t) -> *)
+(*   eval_expr e m v -> *)
+(*   event_step (S, P, Some (COutput Public e), m, t) (OutputEvent v) *)
+(*     (S, P, None, m, EvOutput Public v :: t) *)
+
+(* | POutputSecret : forall S P e m t v, *)
+(*   exec_command (S, P, Some (COutput Secret e), m, t) (S, P, None, m, EvOutput Secret v :: t) -> *)
+(*   eval_expr e m v -> *)
+(*   event_step (S, P, Some (COutput Secret e), m, t) EmptyEvent (S, P, None, m, EvOutput Secret v :: t) *)
+(* . *)
+
+(* Lemma exec_command_iff_event_step : *)
+(*   forall st st', exec_command st st' <-> exists ev, event_step st ev st'. *)
+(* Proof. *)
+(*   intros; split;intros; cycle 1. *)
+(*   - destruct H; induction H; assumption. *)
+(*   - induction H; try (eexists; (econstructor; eauto); (econstructor; eauto)). *)
+(*     + destruct IHexec_command as [ev IHexec_command]. *)
+(*       exists ev ; (econstructor; auto) ; (econstructor; auto). *)
+(*     + destruct IHexec_command as [ev IHexec_command]. *)
+(*       exists ev ; (econstructor; auto) ; (econstructor; auto). *)
+(*     + destruct ch; (eexists; (econstructor; eauto); (econstructor; eauto)). *)
+(* Qed. *)
 
 (* Attempt at defining a statement that intertwines execution and typechecking *)
-Inductive exec_with_gamma : state -> context -> confidentiality -> state -> context -> confidentiality -> Prop :=
-| GSkip : forall S P m t gamma pc,
-    exec_with_gamma (S, P, Some CSkip, m, t) gamma pc (S, P, None, m, t) gamma pc
-| GAssign : forall S P x e v m t gamma pc l gamma',
-    eval_expr e m v ->
-    typecheck_expr gamma e l ->
-    gamma' = set_var x (join l pc) gamma ->
-    exec_with_gamma (S, P, Some (CAssign x e), m, t) gamma pc
-      (S, P, None, set_var x v m, t) gamma' pc
-| GSeq1 : forall S P c1 c2 m t S' P' c1' m' t' gamma pc gamma' pc',
-    exec_with_gamma (S, P, Some c1, m, t) gamma pc (S', P', Some c1', m', t') gamma' pc' ->
-    exec_with_gamma (S, P, Some (CSeq c1 c2), m, t) gamma pc
-      (S', P', Some (CSeq c1' c2), m', t') gamma' pc' (* Should this last one be pc? pc'? *)
-| GSeq2 : forall S P c1 c2 m t S' P' m' t' gamma pc gamma' pc' ,
-    exec_with_gamma (S, P, Some c1, m, t) gamma pc (S', P', None, m', t') gamma' pc' ->
-    exec_with_gamma (S, P, Some (CSeq c1 c2), m, t) gamma pc
-      (S', P', Some c2, m', t') gamma' pc (* This should not be pc', since we are done with c1 and should revert to what we had before *)
-| GIf : forall S P e (c1 : command) c2 m t v (c: command) gamma pc l,
-    eval_expr e m v -> typecheck_expr gamma e l ->
-    c = (if Nat.eqb v 0 then c2 else c1) ->
-    exec_with_gamma (S, P, Some (CIfThenElse e c1 c2), m, t) gamma pc
-      (S, P, Some c, m, t) gamma (join pc l)
-| GWhile : forall S P e c m t gamma pc,
-    exec_with_gamma (S, P, Some (CWhile e c), m, t) gamma pc
-      (S, P, Some (CIfThenElse e (CSeq c (CWhile e c)) CSkip), m, t) gamma pc
-| GInputPublic : forall S v P x m t gamma pc gamma',
-    gamma' = set_var x pc gamma ->
-    exec_with_gamma (S, Streams.Cons v P, Some (CInput Public x), m, t) gamma pc
-      (S, P, None, set_var x v m, EvInput Public v :: t) gamma' pc
-| GInputSecret : forall v S P x m t gamma pc gamma',
-    gamma' = set_var x LSecret gamma ->
-    exec_with_gamma (Streams.Cons v S, P, Some (CInput Secret x), m, t) gamma pc
-      (S, P, None, set_var x v m, EvInput Secret v :: t) gamma' pc
-| GOutput : forall S P ch e m t v gamma pc,
-    eval_expr e m v ->
-    exec_with_gamma (S, P, Some (COutput ch e), m, t) gamma pc
-      (S, P, None, m, EvOutput ch v :: t) gamma pc
+(* Reserved Notation "cfg gamma pc '===>' cfg' gamma' pc'" (at level 10). *)
+Inductive exec_with_gamma : config -> context -> confidentiality -> config -> context -> confidentiality -> Prop :=
+| GSkip : forall st Γ pc,
+  exec_with_gamma
+      (⟪ Some SKIP, st ⟫) Γ pc
+      (⟪ None , st ⟫) Γ pc
+
+| GAssign : forall S P x e v m t Γ pc l Γ',
+  e ; m ⇓ v ->
+  {{ Γ ⊢ e : l }} ->
+  Γ' = <[ x := l ⊔ pc ]> Γ ->
+  exec_with_gamma
+    (⟪ Some (x ::= e), (S, P, m, t) ⟫) Γ pc
+    (⟪ None, (S, P, <[ x := v ]> m, t) ⟫) Γ' pc
+
+| GSeq1 : forall st c1 c2 st' c1' Γ pc Γ' pc',
+    exec_with_gamma
+      (⟪ Some c1, st ⟫) Γ pc
+      (⟪ Some c1', st' ⟫) Γ' pc'
+    ->
+    exec_with_gamma
+      (⟪ Some (c1 ;;; c2), st ⟫) Γ pc
+      (⟪ Some (c1' ;;; c2), st' ⟫) Γ' pc' (* Should this last one be pc? pc'? *)
+
+| GSeq2 : forall st c1 c2 st' Γ pc Γ' pc' ,
+    exec_with_gamma
+      (⟪ Some c1, st ⟫) Γ pc
+      (⟪ None, st' ⟫) Γ' pc'
+    ->
+    exec_with_gamma
+      (⟪ Some (c1 ;;; c2), st ⟫) Γ pc
+      (⟪ Some c2, st' ⟫) Γ' pc'
+      (* This should not be pc', since we are done with c1 and should revert to what we had before *)
+
+| GIf : forall S P e (c1 c2 : command) m t v (c: command) Γ pc l,
+  e ; m ⇓ v ->
+  {{ Γ ⊢ e : l }} ->
+  c = (if Nat.eqb v 0 then c2 else c1) ->
+  exec_with_gamma
+      (⟪ Some (IFB e THEN c1 ELSE c2 FI),  (S, P, m, t)⟫) Γ pc
+      (⟪ Some c,  (S, P, m, t)⟫) Γ (pc ⊔ l)
+
+| GWhile : forall st e c Γ pc,
+    exec_with_gamma
+      (⟪ Some (WHILE e DO c END), st ⟫) Γ pc
+      (⟪ Some (IFB e THEN (c ;;; WHILE e DO c END) ELSE SKIP FI), st ⟫) Γ pc
+
+| GInputPublic : forall S v P x m t Γ pc Γ',
+    Γ' = <[ x := pc ]> Γ ->
+    exec_with_gamma
+      (⟪ Some (INPUT x @Public), (S, v::::P, m, t) ⟫) Γ pc
+      (⟪ None, (S, P, <[x := v ]> m, EvInput Public v :: t) ⟫) Γ' pc
+
+| GInputSecret : forall S v P x m t Γ pc Γ',
+    Γ' = <[ x := LSecret ]> Γ ->
+    exec_with_gamma
+      (⟪ Some (INPUT x @Secret), (v::::S, P, m, t) ⟫) Γ pc
+      (⟪ None, (S, P, <[x := v ]> m, EvInput Secret v :: t) ⟫) Γ' pc
+
+| GOutput : forall S P ch e m t v Γ pc,
+  e ; m ⇓ v ->
+    exec_with_gamma
+      (⟪ Some (OUTPUT e @ch), (S, P, m, t) ⟫) Γ pc
+      (⟪ None, (S, P, m, EvOutput ch v :: t) ⟫) Γ pc
 .
 
-
-Inductive exec_with_gamma_trans : state -> context -> confidentiality -> state -> context -> confidentiality -> Prop :=
+Inductive exec_with_gamma_trans : config -> context -> confidentiality -> config -> context -> confidentiality -> Prop :=
 | Gexec_empty : forall s gamma pc, exec_with_gamma_trans s gamma pc s gamma pc
 | Gexec_step : forall s1 gamma1 pc1 s2 gamma2 pc2 s3 gamma3 pc3,
     exec_with_gamma s1 gamma1 pc1 s2 gamma2 pc2 ->
@@ -530,9 +712,9 @@ Inductive exec_with_gamma_trans : state -> context -> confidentiality -> state -
 
 
 (* Two memories have the same values for the public variables *)
-Definition agree_on_public (gamma : context) (m1 m2 : memory) : Prop :=
+Definition agree_on_public (Γ : context) (m1 m2 : memory) : Prop :=
   forall x,
-    match find_var x m1, find_var x m2, find_var x gamma with
+    match m1 !! x, m2 !! x, Γ !! x with
     | Some v1, Some v2, Some LPublic => v1 = v2
     | _, _, Some LSecret => True
     | None, None, None => True
@@ -553,7 +735,7 @@ Definition agree_on_public (gamma : context) (m1 m2 : memory) : Prop :=
    induction e; intros v2 v1 Ht Hagree Hv1 Hv2.
    - inversion Hv1; subst. inversion Hv2; subst. done.
    - inversion Hv1; subst. inversion Hv2; subst. inversion Ht; subst.
-     specialize (Hagree v). rewrite H0 H1 H3 in Hagree. done.
+     specialize (Hagree s). rewrite H0 H1 H3 in Hagree. done.
    - inversion Hv1; subst. inversion Hv2; subst.
      inversion Ht; subst. destruct l1 => //. destruct l2 => //.
      rewrite (IHe1 v1 v0 H3 Hagree H4 H6).
@@ -562,23 +744,60 @@ Definition agree_on_public (gamma : context) (m1 m2 : memory) : Prop :=
 
 
 (* executing implies executing with gammas *)
-Lemma can_exec_with_gamma gamma0 pc0 P0 S0 c0 m0 t0 s1 :
-  same_support m0 gamma0 ->
-  exec_trans (P0, S0, c0, m0, t0) s1 ->
-  exists gamma1 pc1, exec_with_gamma_trans (P0, S0, c0, m0, t0) gamma0 pc0 s1 gamma1 pc1.
+Lemma can_exec_with_gamma Γ0 pc0 P0 S0 c0 m0 t0 s1 :
+  same_support m0 Γ0 ->
+  (⟪ c0 , (P0, S0, m0, t0) ⟫) ---> s1 ->
+  exists Γ1 pc1,
+    exec_with_gamma
+      (⟪ c0 , (P0, S0, m0, t0) ⟫) Γ0 pc0
+      s1 Γ1 pc1.
 Proof.
+  intros Hwf Hstep.
+  destruct c0 as [c0|]; [|by inversion Hstep].
+  induction Hstep; subst
+  ; try ( eexists _,_; econstructor ; eauto; done).
+  - admit.
+    (* destruct H6. *)
+    (* + exists (<[ x := pc0 ]> Γ0), pc0. *)
+    (*   repeat econstructor. by destruct pc0 ; cbn. *)
+    (* + admit. (* need more information about m *) *)
+    (* + admit. *)
+  - destruct IHHstep as (Γ1 & pc1 & IH).
+    eexists _,_; econstructor ; eauto.
+  - destruct IHHstep as (Γ1 & pc1 & IH).
+    eexists _,_; econstructor ; eauto.
+  - (* need more information about m *)
+    admit.
 Admitted.
 
-
-
-
+(* executing implies executing with gammas *)
+Lemma can_exec_with_gamma_trans Γ0 pc0 P0 S0 c0 m0 t0 s1 :
+  same_support m0 Γ0 ->
+  (⟪ c0 , (P0, S0, m0, t0) ⟫) --->* s1 ->
+  exists Γ1 pc1,
+    exec_with_gamma_trans
+      (⟪ c0 , (P0, S0, m0, t0) ⟫) Γ0 pc0
+      s1 Γ1 pc1.
+Proof.
+  intros Hwf Hstep.
+  induction Hstep.
+  - eexists; eexists; econstructor.
+  - destruct IHHstep as (Γ1 & pc1 & IH).
+    (* destruct x,st. as (S & P & m & t). *)
+    destruct x,st,p,p.
+    eapply can_exec_with_gamma in Hwf.
+    + admit.
+    + admit.
+Admitted.
 
 Lemma type_preservation :
   forall c gamma pc gammaf gamma' P S m t P' S' c' m' t' pc',
-  typecheck gamma pc c gammaf ->
-  exec_with_gamma (P, S, Some c, m, t) gamma pc (P', S', c', m', t') gamma' pc' ->
+  -{ gamma, pc ⊢ c ~> gammaf }- ->
+  exec_with_gamma
+    (⟪ Some c , (S, P, m, t) ⟫) gamma pc
+    (⟪ c' , (S', P', m', t') ⟫) gamma' pc' ->
   match c' with
-    Some c' => typecheck gamma' pc' c' gammaf
+  | Some c' => -{ gamma', pc' ⊢ c' ~> gammaf }-
   | None => gamma' = gammaf
   end .
 Proof.
@@ -588,8 +807,8 @@ Proof.
   - inversion Ht; subst. replace l with le => //.
     admit.
   - inversion Ht; subst.
-    specialize (IHc1 _ _ _ _ _ _ _ _ _ _ _ _ _ _ H3 H14).
-    eapply TSeq. exact IHc1.
+    (* specialize (IHc1 _ _ _ _ _ _ _ _ _ _ _ _ _ _ H3). *)
+    (* eapply TSeq. exact IHc1. *)
 
 (* For the end of this proof to work, we need to tweak our definition of
    exec_with_gamma *)
@@ -625,36 +844,41 @@ Admitted. *)
 (* One can separate an execution into its last event, everything that happens before,
 and everything that happens after *)
 Lemma separate_last_event S0 P0 c0 m0 t0 gamma0 pc0 S1 P1 c1 m1 a t1 gamma1 pc1 :
-  exec_with_gamma_trans (S0, P0, Some c0, m0, t0) gamma0 pc0
-    (S1, P1, c1, m1, a :: t1) gamma1 pc1 ->
+  exec_with_gamma_trans
+    (⟪ Some c0 , (S0, P0, m0, t0) ⟫) gamma0 pc0
+    (⟪ c1 , (S1, P1, m1, a::t1) ⟫) gamma1 pc1 ->
   exists S2 P2 c2 m2 gamma2 pc2 S3 P3 c3 m3 gamma3 pc3,
-    exec_with_gamma_trans (S0, P0, Some c0, m0, t0) gamma0 pc0
-      (S2, P2, Some c2, m2, t1) gamma2 pc2 /\
-      exec_with_gamma (S2, P2, Some c2, m2, t1) gamma2 pc2
-        (S3, P3, c3, m3, a :: t1) gamma3 pc3 /\
-      exec_with_gamma_trans (S3, P3, c3, m3, a :: t1) gamma3 pc3
-        (S1, P1, c1, m1, a :: t1) gamma1 pc1.
+    exec_with_gamma_trans
+    (⟪ Some c0 , (S0, P0, m0, t0) ⟫) gamma0 pc0
+    (⟪ Some c2 , (S2, P2, m2, t1) ⟫) gamma2 pc2
+    /\ exec_with_gamma
+        (⟪ Some c2 , (S2, P2, m2, t1) ⟫) gamma2 pc2
+        (⟪ c3 , (S3, P3, m3, a::t1) ⟫) gamma3 pc3
+    /\ exec_with_gamma_trans
+        (⟪ c3 , (S3, P3, m3, a::t1) ⟫) gamma3 pc3
+        (⟪ c1 , (S1, P1, m1, a::t1) ⟫) gamma1 pc1.
 Proof.
 Admitted.
-
 
 (* Same as the previous lemma, but with public events only *)
 Lemma separate_last_public_event S0 P0 c0 m0 t0 gamma0 pc0 S1 P1 c1 m1 t1 a d gamma1 pc1:
-  exec_with_gamma_trans (S0, P0, Some c0, m0, t0) gamma0 pc0
-    (S1, P1, c1, m1, t1) gamma1 pc1 ->
+  exec_with_gamma_trans
+    (⟪ Some c0 , (S0, P0, m0, t0) ⟫) gamma0 pc0
+    (⟪ c1 , (S1, P1, m1, t1) ⟫) gamma1 pc1 ->
   public_projection t1 = a :: d ->
   exists S2 P2 c2 m2 t2 gamma2 pc2 S3 P3 c3 m3 gamma3 pc3,
-    exec_with_gamma_trans (S0, P0, Some c0, m0, t0) gamma0 pc0
-      (S2, P2, Some c2, m2, t2) gamma2 pc2 /\
-      public_projection t2 = d /\
-      exec_with_gamma  (S2, P2, Some c2, m2, t2) gamma2 pc2
-        (S3, P3, c3, m3, a :: t2) gamma3 pc3 /\
-      exec_with_gamma_trans (S3, P3, c3, m3, a :: t2) gamma3 pc3
-        (S1, P1, c1, m1, t1) gamma1 pc1.
+    exec_with_gamma_trans
+    (⟪ Some c0 , (S0, P0, m0, t0) ⟫) gamma0 pc0
+    (⟪ Some c2 , (S2, P2, m2, t2) ⟫) gamma2 pc2
+    /\ public_projection t2 = d
+    /\ exec_with_gamma
+        (⟪ Some c2 , (S2, P2, m2, t2) ⟫) gamma2 pc2
+        (⟪ c3 , (S3, P3, m3, a::t2) ⟫) gamma3 pc3
+    /\ exec_with_gamma_trans
+        (⟪  c3 , (S3, P3, m3, a::t2) ⟫) gamma3 pc3
+        (⟪ c1 , (S1, P1, m1, t1) ⟫) gamma1 pc1.
 Proof.
 Admitted.
-
-
 
 (* One can add a public event to both sides of a public projection *)
 Lemma public_projection_cons t a d t' d':
@@ -682,10 +906,14 @@ Qed.
 (* if c executes to Some c', then it cannot execute to None *)
 Lemma exec_both_some S1 P1 c m1 t1 gamma1 pc1 S1' P1' c1' m1' t1' gamma1' pc1'
   S2 P2 m2 t2 gamma2 pc2 S2' P2' c2' m2' t2' gamma2' pc2':
-  exec_with_gamma (S1, P1, Some c, m1, t1) gamma1 pc1
-    (S1', P1', c1', m1', t1') gamma1' pc1' ->
-  exec_with_gamma (S2, P2, Some c, m2, t2) gamma2 pc2
-    (S2', P2', c2', m2', t2') gamma2' pc2' ->
+  exec_with_gamma
+    (⟪ Some c , (S1, P1, m1, t1) ⟫) gamma1 pc1
+    (⟪ c1' , (S1', P1', m1', t1') ⟫) gamma1' pc1' ->
+
+  exec_with_gamma
+    (⟪ Some c , (S2, P2, m2, t2) ⟫) gamma2 pc2
+    (⟪ c2' , (S2', P2', m2', t2') ⟫) gamma2' pc2' ->
+
   match c1', c2' with | Some _, Some _ | None, None => True | _,_ => False end.
 Proof.
   intros Hex1 Hex2.
@@ -693,47 +921,21 @@ Proof.
     inversion Hex2; subst => //.
 Qed.
 
-
-Lemma find_set_var {A} x (v : A) l :
-  find_var x (set_var x v l) = Some v.
-Proof.
-  induction l => //=. rewrite String.eqb_refl. done.
-  destruct (v0 =? x) eqn:Hvx => //=. rewrite String.eqb_refl. done.
-  rewrite Hvx. done.
-Qed.
-
-Lemma find_set_var_diff {A} x y (v : A) l :
-  x <> y ->
-  find_var y (set_var x v l) = find_var y l.
-Proof.
-  intro Hxy. apply String.eqb_neq in Hxy.
-  induction l => //=. by rewrite Hxy.
-  destruct (v0 =? x) eqn:Hvx => //=.
-  rewrite Hxy.   destruct (v0 =? y) eqn:Hvy => //=.
-  apply String.eqb_eq in Hvy, Hvx; subst. rewrite String.eqb_neq in Hxy. done.
-  by rewrite IHl.
-Qed.
-
-
-
- Lemma set_var_agree gamma (m1 m2 : memory) x v l :
+Lemma set_var_agree gamma (m1 m2 : memory) x v l :
   agree_on_public gamma m1 m2 ->
-  agree_on_public (set_var x l gamma) (set_var x v m1) (set_var x v m2).
- Proof.
-   unfold agree_on_public.
-   intros Hagree y.
-   destruct (x =? y) eqn:Hxy.
-   - apply String.eqb_eq in Hxy as ->.
-     repeat rewrite find_set_var. by destruct l.
-   - apply String.eqb_neq in Hxy.
-     rewrite find_set_var_diff => //.
-     rewrite find_set_var_diff => //.
-     rewrite find_set_var_diff => //.
-     by apply Hagree.
- Qed.
-
-
-
+  agree_on_public (<[ x := l ]> gamma)
+    (<[ x := v ]> m1)
+    (<[ x := v ]> m2).
+Proof.
+  unfold agree_on_public.
+  intros Hagree y.
+  destruct (x =? y) eqn:Hxy.
+  - apply String.eqb_eq in Hxy as ->.
+    simpl_map; by destruct l.
+  - apply String.eqb_neq in Hxy.
+    repeat (rewrite lookup_insert_ne => //).
+    apply Hagree.
+Qed.
 
 (* If a step produces a public event, then it is observationally deterministic *)
 Lemma public_event_is_same :
@@ -745,10 +947,12 @@ Lemma public_event_is_same :
   public_projection (a1 :: t1) = a1 :: d ->
   public_projection (a2 :: t2) = a2 :: d ->
   agree_on_public gamma m1 m2 ->
-  exec_with_gamma (S1, P, Some c, m1, t1) gamma pc
-    (S1', P1', c1', m1', a1 :: t1) gamma1 pc1 ->
-  exec_with_gamma (S2, P, Some c, m2, t2) gamma pc
-    (S2', P2', c2', m2', a2 :: t2) gamma2 pc2 ->
+  exec_with_gamma
+    (⟪ Some c , (S1, P, m1, t1) ⟫) gamma pc
+    (⟪ c1' , (S1', P1', m1', a1 :: t1) ⟫) gamma1 pc1 ->
+  exec_with_gamma
+    (⟪ Some c , (S2, P, m2, t2) ⟫) gamma pc
+    (⟪ c2' , (S2', P2', m2', a2:: t2) ⟫) gamma2 pc2 ->
   gamma1 = gamma2 /\ pc1 = pc2 /\ P1' = P2' /\ c1' = c2' /\ agree_on_public gamma1 m1' m2' /\ a1 = a2.
 Proof.
   induction c;
@@ -760,16 +964,16 @@ Proof.
       * inversion Ht.
         assert (public_projection t1 = public_projection t1) as Htriv => //.
         edestruct (IHc1 _ _ _ _ _ _ _ _ _ _ _ _ _ _ _ _ _ _ _ _ _ _ _ _ _
-                     H3 Htriv Ht2 Ha1 Ha2 Hmem H14 H15)
+                     H3 Htriv Ht2 Ha1 Ha2 Hmem H8 H9)
           as (-> & -> & -> & ? & ? & ->).
         inversion H6; subst. by repeat split.
-      * eapply exec_both_some in H14; try exact H15. done.
+      * eapply exec_both_some in H8; try exact H9. done.
     + inversion Hex2; subst.
-      * eapply exec_both_some in H14; try exact H15. done.
+      * eapply exec_both_some in H8; try exact H9. done.
       * inversion Ht.
         assert (public_projection t1 = public_projection t1) as Htriv => //.
         edestruct (IHc1 _ _ _ _ _ _ _ _ _ _ _ _ _ _ _ _ _ _ _ _ _ _ _ _ _
-                     H3 Htriv Ht2 Ha1 Ha2 Hmem H14 H15)
+                     H3 Htriv Ht2 Ha1 Ha2 Hmem H8 H9)
           as (-> & -> & -> & ? & ? & ->).
         done.
   - inversion Hex1; subst.
@@ -816,18 +1020,23 @@ Lemma identical_after_nth_public_event :
   forall d1 a1 a2 d2 c gamma Sinit1 P S1 P1 c1 m1 t1 gamma1 pc1 S1' P1' c1' m1' gamma1' pc1'
     Sinit2 S2 P2 c2 m2 t2 gamma2 pc2 S2' P2' c2' m2' gamma2' pc2',
     length d1 = length d2 ->
-    typecheck gamma0 LPublic c gamma ->
-    exec_with_gamma_trans (Sinit1, P, Some c, minit, nil) gamma0 LPublic
-      (S1, P1, Some c1, m1, t1) gamma1 pc1 ->
+    -{ gamma0 , LPublic ⊢ c ~> gamma }- ->
+    (* typecheck gamma0 LPublic c gamma -> *)
+    exec_with_gamma_trans
+      (⟪ Some c , (Sinit1, P, minit, []) ⟫) gamma0 LPublic
+      (⟪ Some c1 , (S1, P1, m1, t1) ⟫) gamma1 pc1 ->
     public_projection t1 = d1 ->
-    exec_with_gamma (S1, P1, Some c1, m1, t1) gamma1 pc1
-      (S1', P1', c1', m1', a1 :: t1) gamma1' pc1' ->
+    exec_with_gamma
+      (⟪ Some c1 , (S1, P1, m1, t1) ⟫) gamma1 pc1
+      (⟪ c1' , (S1', P1', m1', a1 :: t1) ⟫) gamma1' pc1' ->
     public_projection (a1 :: t1) = a1 :: d1 ->
-    exec_with_gamma_trans (Sinit2, P, Some c, minit, nil) gamma0 LPublic
-      (S2, P2, Some c2, m2, t2) gamma2 pc2 ->
+    exec_with_gamma_trans
+      (⟪ Some c , (Sinit2, P, minit, []) ⟫) gamma0 LPublic
+      (⟪ Some c2 , (S2, P2, m2, t2) ⟫) gamma2 pc2 ->
     public_projection t2 = d2 ->
-    exec_with_gamma (S2, P2, Some c2, m2, t2) gamma2 pc2
-      (S2', P2', c2', m2', a2 :: t2) gamma2' pc2' ->
+    exec_with_gamma
+      (⟪ Some c2 , (S2, P2, m2, t2) ⟫) gamma2 pc2
+      (⟪ c2' , (S2', P2', m2', a2 :: t2) ⟫) gamma2' pc2' ->
     public_projection (a2 :: t2) = a2 :: d2 ->
     gamma1 = gamma2 /\ pc1 = pc2 /\ P1 = P2 /\ c1 = c2 /\ agree_on_public gamma1 m1 m2 /\ a1 = a2 /\ d1 = d2.
 Proof.
@@ -864,6 +1073,8 @@ Admitted.
 
 
 
+
+
 Lemma typecheck_is_sound :
   forall c gamma, typecheck gamma0 LPublic c gamma -> PINI c.
 Proof.
@@ -882,12 +1093,12 @@ Proof.
   destruct H as (S' & P' & c' & m' & t' & a0 & Hexec & Hp0).
   destruct Had as (S0 & S1 & P1 & c1 & m1 & Hexec0 & Hp).
   replace a with a0. exists S', P',c', m', t'. split => //.
-  apply (can_exec_with_gamma gamma0 LPublic) in Hexec0 as (gamma1 & pc1 & Hexec0);
+  apply (can_exec_with_gamma_trans gamma0 LPublic) in Hexec0 as (gamma1 & pc1 & Hexec0);
     last done.
   destruct (separate_last_public_event _ _ _ _ _ _ _ _ _ _ _ _ _ _ _ _ Hexec0 Hp)
     as (S1m & P1m & c1m & m1m & t1m & gamma1m & pc1m &
           S1p & P1p & c1p & m1p & gamma1p & pc1p & Hex1m & Ht1m & Hex1c & Hex1p).
-  apply (can_exec_with_gamma gamma0 LPublic) in Hexec as (gamma2 & pc2 & Hexec);
+  apply (can_exec_with_gamma_trans gamma0 LPublic) in Hexec as (gamma2 & pc2 & Hexec);
     last done.
   destruct (separate_last_public_event _ _ _ _ _ _ _ _ _ _ _ _ _ _ _ _ Hexec Hp0)
     as (S2m & P2m & c2m & m2m & t2m & gamma2m & pc2m &
@@ -905,5 +1116,3 @@ Proof.
   exact Hex2c.
   by apply (public_projection_cons _ _ _ _ _ Hp0 Ht2m).
 Qed.
-
-
